Improve adherence to the style guide's naming conventions

ironfleet/src/Dafny/Distributed/Impl/Common/GenericRefinement.i.dfy
@@ -31,7 +31,7 @@ predicate MapIsAbstractable<KT,VT,CKT,CVT>(m:map<CKT,CVT>, RefineKey:CKT->KT, Re
     && (forall ck :: ck in m ==> ReverseKey.requires(RefineKey(ck)) && ReverseKey(RefineKey(ck)) == ck)
 }
 
-function {:opaque} RefineToMap<CKT,CVT,KT,VT>(m:map<CKT,CVT>, RefineKey:CKT->KT, RefineValue:CVT->VT, ReverseKey:KT->CKT) : map<KT,VT>
+function {:opaque} AbstractifyMap<CKT,CVT,KT,VT>(m:map<CKT,CVT>, RefineKey:CKT->KT, RefineValue:CVT->VT, ReverseKey:KT->CKT) : map<KT,VT>
     reads RefineKey.reads, RefineValue.reads, ReverseKey.reads;
     requires forall ck :: ck in m ==> RefineKey.requires(ck) && RefineValue.requires(m[ck]);
     requires forall ck :: ck in m ==> ReverseKey.requires(RefineKey(ck)) && ReverseKey(RefineKey(ck)) == ck;
@@ -40,34 +40,34 @@ function {:opaque} RefineToMap<CKT,CVT,KT,VT>(m:map<CKT,CVT>, RefineKey:CKT->KT,
     map k | k in new_domain :: RefineValue(m[ReverseKey(k)])
 }
 
-lemma lemma_RefineToMap_basic_properties<CKT,CVT,KT,VT>(m:map<CKT,CVT>, RefineKey:CKT->KT, RefineValue:CVT->VT, ReverseKey:KT->CKT)
+lemma Lemma_AbstractifyMap_basic_properties<CKT,CVT,KT,VT>(m:map<CKT,CVT>, RefineKey:CKT->KT, RefineValue:CVT->VT, ReverseKey:KT->CKT)
     requires MapIsAbstractable(m, RefineKey, RefineValue, ReverseKey);
     // Injectivity
     requires forall ck1, ck2 :: RefineKey.requires(ck1) && RefineKey.requires(ck2) && RefineKey(ck1) == RefineKey(ck2) ==> ck1 == ck2;
-    ensures  m == map [] ==> RefineToMap(m, RefineKey, RefineValue, ReverseKey) == map [];
-    ensures  forall ck :: ck in m <==> RefineKey.requires(ck) && RefineKey(ck) in RefineToMap(m, RefineKey, RefineValue, ReverseKey);
-    ensures  forall ck :: ck in m ==> RefineToMap(m, RefineKey, RefineValue, ReverseKey)[RefineKey(ck)] == RefineValue(m[ck]);
+    ensures  m == map [] ==> AbstractifyMap(m, RefineKey, RefineValue, ReverseKey) == map [];
+    ensures  forall ck :: ck in m <==> RefineKey.requires(ck) && RefineKey(ck) in AbstractifyMap(m, RefineKey, RefineValue, ReverseKey);
+    ensures  forall ck :: ck in m ==> AbstractifyMap(m, RefineKey, RefineValue, ReverseKey)[RefineKey(ck)] == RefineValue(m[ck]);
 {
-    reveal_RefineToMap();
+    reveal_AbstractifyMap();
 }
 
-lemma lemma_RefineToMap_preimage<KT,VT,CKT,CVT>(cm:map<CKT,CVT>, RefineKey:CKT->KT, RefineValue:CVT->VT, ReverseKey:KT->CKT)
+lemma Lemma_AbstractifyMap_preimage<KT,VT,CKT,CVT>(cm:map<CKT,CVT>, RefineKey:CKT->KT, RefineValue:CVT->VT, ReverseKey:KT->CKT)
     requires MapIsAbstractable(cm, RefineKey, RefineValue, ReverseKey);
     // Injectivity
     requires forall ck1, ck2 :: RefineKey.requires(ck1) && RefineKey.requires(ck2) && RefineKey(ck1) == RefineKey(ck2) ==> ck1 == ck2;
-    ensures  var rm  := RefineToMap(cm, RefineKey, RefineValue, ReverseKey);
+    ensures  var rm  := AbstractifyMap(cm, RefineKey, RefineValue, ReverseKey);
              forall k :: k in rm ==> (exists ck :: ck in cm && RefineKey(ck) == k);
 {
-    var rm  := RefineToMap(cm, RefineKey, RefineValue, ReverseKey);
-    lemma_RefineToMap_basic_properties(cm, RefineKey, RefineValue, ReverseKey);
+    var rm  := AbstractifyMap(cm, RefineKey, RefineValue, ReverseKey);
+    Lemma_AbstractifyMap_basic_properties(cm, RefineKey, RefineValue, ReverseKey);
     forall k | k in rm 
         ensures (exists ck :: ck in cm && RefineKey(ck) == k);
     {
-        reveal_RefineToMap();
+        reveal_AbstractifyMap();
     }
 }
 
-lemma lemma_RefineToMap_append<KT,VT,CKT,CVT>(cm:map<CKT,CVT>, 
+lemma Lemma_AbstractifyMap_append<KT,VT,CKT,CVT>(cm:map<CKT,CVT>, 
                                RefineKey:CKT->KT, RefineValue:CVT->VT, ReverseKey:KT->CKT,
                                ck:CKT, cval:CVT)
     requires MapIsAbstractable(cm, RefineKey, RefineValue, ReverseKey);
@@ -76,28 +76,28 @@ lemma lemma_RefineToMap_append<KT,VT,CKT,CVT>(cm:map<CKT,CVT>,
     requires RefineKey.requires(ck);
     requires RefineValue.requires(cval);
     requires ReverseKey.requires(RefineKey(ck)) && ReverseKey(RefineKey(ck)) == ck;
-    ensures  var rm  := RefineToMap(cm, RefineKey, RefineValue, ReverseKey);
-             var rm' := RefineToMap(cm[ck := cval], RefineKey, RefineValue, ReverseKey);
-             rm' == RefineToMap(cm, RefineKey, RefineValue, ReverseKey)[RefineKey(ck) := RefineValue(cval)];
+    ensures  var rm  := AbstractifyMap(cm, RefineKey, RefineValue, ReverseKey);
+             var rm' := AbstractifyMap(cm[ck := cval], RefineKey, RefineValue, ReverseKey);
+             rm' == AbstractifyMap(cm, RefineKey, RefineValue, ReverseKey)[RefineKey(ck) := RefineValue(cval)];
 {
-    var rm := RefineToMap(cm, RefineKey, RefineValue, ReverseKey);
+    var rm := AbstractifyMap(cm, RefineKey, RefineValue, ReverseKey);
     var cm' := cm[ck := cval];
-    var rm' := RefineToMap(cm', RefineKey, RefineValue, ReverseKey);
-    var r_cm' := RefineToMap(cm, RefineKey, RefineValue, ReverseKey)[RefineKey(ck) := RefineValue(cval)];
+    var rm' := AbstractifyMap(cm', RefineKey, RefineValue, ReverseKey);
+    var r_cm' := AbstractifyMap(cm, RefineKey, RefineValue, ReverseKey)[RefineKey(ck) := RefineValue(cval)];
 
     forall rk | rk in rm'
         ensures rk in r_cm';
         ensures r_cm'[rk] == rm'[rk];
     {
-        lemma_RefineToMap_basic_properties(cm', RefineKey, RefineValue, ReverseKey);
-        lemma_RefineToMap_preimage(cm', RefineKey, RefineValue, ReverseKey);
+        Lemma_AbstractifyMap_basic_properties(cm', RefineKey, RefineValue, ReverseKey);
+        Lemma_AbstractifyMap_preimage(cm', RefineKey, RefineValue, ReverseKey);
         var preimage :| preimage in cm' && RefineKey(preimage) == rk;
 
         if preimage in cm {
-            lemma_RefineToMap_basic_properties(cm, RefineKey, RefineValue, ReverseKey);
+            Lemma_AbstractifyMap_basic_properties(cm, RefineKey, RefineValue, ReverseKey);
             calc ==> {
                 true;
-                { lemma_RefineToMap_preimage(cm, RefineKey, RefineValue, ReverseKey); }
+                { Lemma_AbstractifyMap_preimage(cm, RefineKey, RefineValue, ReverseKey); }
                 RefineKey(preimage) in rm;
                 RefineKey(preimage) in rm';
                 rk in r_cm';
@@ -106,15 +106,15 @@ lemma lemma_RefineToMap_append<KT,VT,CKT,CVT>(cm:map<CKT,CVT>,
             assert preimage == ck;
             assert RefineKey(preimage) in r_cm';
         }
-        reveal_RefineToMap();
+        reveal_AbstractifyMap();
     }
 
     forall rk | rk in r_cm'
         ensures rk in rm';
     {
-        lemma_RefineToMap_basic_properties(cm, RefineKey, RefineValue, ReverseKey);
-        lemma_RefineToMap_preimage(cm, RefineKey, RefineValue, ReverseKey);
-        lemma_RefineToMap_basic_properties(cm', RefineKey, RefineValue, ReverseKey);
+        Lemma_AbstractifyMap_basic_properties(cm, RefineKey, RefineValue, ReverseKey);
+        Lemma_AbstractifyMap_preimage(cm, RefineKey, RefineValue, ReverseKey);
+        Lemma_AbstractifyMap_basic_properties(cm', RefineKey, RefineValue, ReverseKey);
         if rk in rm {
             var preimage :| preimage in cm && RefineKey(preimage) == rk;
             assert rk in rm';
@@ -126,7 +126,7 @@ lemma lemma_RefineToMap_append<KT,VT,CKT,CVT>(cm:map<CKT,CVT>,
     assert r_cm' == rm';
 }
 
-lemma lemma_RefineToMap_remove<KT,VT,CKT,CVT>(cm:map<CKT,CVT>, 
+lemma Lemma_AbstractifyMap_remove<KT,VT,CKT,CVT>(cm:map<CKT,CVT>, 
                                RefineKey:CKT->KT, RefineValue:CVT->VT, ReverseKey:KT->CKT,
                                ck:CKT)
     requires MapIsAbstractable(cm, RefineKey, RefineValue, ReverseKey);
@@ -135,24 +135,24 @@ lemma lemma_RefineToMap_remove<KT,VT,CKT,CVT>(cm:map<CKT,CVT>,
     requires RefineKey.requires(ck);
     requires ReverseKey.requires(RefineKey(ck)) && ReverseKey(RefineKey(ck)) == ck;
     requires ck in cm;
-    ensures  var rm  := RefineToMap(cm, RefineKey, RefineValue, ReverseKey);
-             var rm' := RefineToMap(RemoveElt(cm, ck), RefineKey, RefineValue, ReverseKey);
+    ensures  var rm  := AbstractifyMap(cm, RefineKey, RefineValue, ReverseKey);
+             var rm' := AbstractifyMap(RemoveElt(cm, ck), RefineKey, RefineValue, ReverseKey);
              RefineKey(ck) in rm &&
              rm' == RemoveElt(rm, RefineKey(ck));
 {
-    lemma_RefineToMap_basic_properties(cm, RefineKey, RefineValue, ReverseKey);
+    Lemma_AbstractifyMap_basic_properties(cm, RefineKey, RefineValue, ReverseKey);
 
-    var rm  := RefineToMap(cm, RefineKey, RefineValue, ReverseKey);
+    var rm  := AbstractifyMap(cm, RefineKey, RefineValue, ReverseKey);
     var smaller_cm := RemoveElt(cm, ck);
-    var rm' := RefineToMap(smaller_cm, RefineKey, RefineValue, ReverseKey);
+    var rm' := AbstractifyMap(smaller_cm, RefineKey, RefineValue, ReverseKey);
     var smaller_rm := RemoveElt(rm, RefineKey(ck));
 
-    lemma_RefineToMap_basic_properties(smaller_cm, RefineKey, RefineValue, ReverseKey);
+    Lemma_AbstractifyMap_basic_properties(smaller_cm, RefineKey, RefineValue, ReverseKey);
 
     forall o | o in rm'
         ensures o in smaller_rm && rm'[o] == smaller_rm[o];
     {
-        lemma_RefineToMap_preimage(smaller_cm, RefineKey, RefineValue, ReverseKey);
+        Lemma_AbstractifyMap_preimage(smaller_cm, RefineKey, RefineValue, ReverseKey);
         var co :| co in smaller_cm && RefineKey(co) == o;
         assert co != ck;
         assert RefineKey(co) != RefineKey(ck);
@@ -161,7 +161,7 @@ lemma lemma_RefineToMap_remove<KT,VT,CKT,CVT>(cm:map<CKT,CVT>,
     forall o | o in smaller_rm
         ensures o in rm' && rm'[o] == smaller_rm[o];
     {
-        lemma_RefineToMap_preimage(cm, RefineKey, RefineValue, ReverseKey);
+        Lemma_AbstractifyMap_preimage(cm, RefineKey, RefineValue, ReverseKey);
         var co :| co in cm && co != ck && RefineKey(co) == o;
     }
 
@@ -169,45 +169,45 @@ lemma lemma_RefineToMap_remove<KT,VT,CKT,CVT>(cm:map<CKT,CVT>,
     assert rm' == smaller_rm;
 }
 
-lemma lemma_RefineToMap_properties<CKT,CVT,KT,VT>(cm:map<CKT,CVT>, RefineKey:CKT->KT, RefineValue:CVT->VT, ReverseKey:KT->CKT)
+lemma lemma_AbstractifyMap_properties<CKT,CVT,KT,VT>(cm:map<CKT,CVT>, RefineKey:CKT->KT, RefineValue:CVT->VT, ReverseKey:KT->CKT)
     requires MapIsAbstractable(cm, RefineKey, RefineValue, ReverseKey);
     // Injectivity
     requires forall ck1, ck2 :: RefineKey.requires(ck1) && RefineKey.requires(ck2) && RefineKey(ck1) == RefineKey(ck2) ==> ck1 == ck2;
-    ensures  cm == map [] ==> RefineToMap(cm, RefineKey, RefineValue, ReverseKey) == map [];
-    ensures  forall ck :: ck in cm <==> RefineKey.requires(ck) && RefineKey(ck) in RefineToMap(cm, RefineKey, RefineValue, ReverseKey);
-    ensures  forall ck :: ck in cm ==> RefineToMap(cm, RefineKey, RefineValue, ReverseKey)[RefineKey(ck)] == RefineValue(cm[ck]);
-    ensures  forall ck :: ck !in cm && RefineKey.requires(ck) ==> RefineKey(ck) !in RefineToMap(cm, RefineKey, RefineValue, ReverseKey);
-    ensures  var rm  := RefineToMap(cm, RefineKey, RefineValue, ReverseKey);
+    ensures  cm == map [] ==> AbstractifyMap(cm, RefineKey, RefineValue, ReverseKey) == map [];
+    ensures  forall ck :: ck in cm <==> RefineKey.requires(ck) && RefineKey(ck) in AbstractifyMap(cm, RefineKey, RefineValue, ReverseKey);
+    ensures  forall ck :: ck in cm ==> AbstractifyMap(cm, RefineKey, RefineValue, ReverseKey)[RefineKey(ck)] == RefineValue(cm[ck]);
+    ensures  forall ck :: ck !in cm && RefineKey.requires(ck) ==> RefineKey(ck) !in AbstractifyMap(cm, RefineKey, RefineValue, ReverseKey);
+    ensures  var rm  := AbstractifyMap(cm, RefineKey, RefineValue, ReverseKey);
              forall k :: k in rm ==> (exists ck :: ck in cm && RefineKey(ck) == k);
     ensures forall ck, cval :: (RefineKey.requires(ck) && RefineValue.requires(cval) 
                                 && ReverseKey.requires(RefineKey(ck)) && ReverseKey(RefineKey(ck)) == ck) ==>
-            var rm  := RefineToMap(cm, RefineKey, RefineValue, ReverseKey);
-            var rm' := RefineToMap(cm[ck := cval], RefineKey, RefineValue, ReverseKey);
-            rm' == RefineToMap(cm, RefineKey, RefineValue, ReverseKey)[RefineKey(ck) := RefineValue(cval)];
-    ensures forall ck {:trigger RemoveElt(RefineToMap(cm, RefineKey, RefineValue, ReverseKey), RefineKey(ck)) } :: 
+            var rm  := AbstractifyMap(cm, RefineKey, RefineValue, ReverseKey);
+            var rm' := AbstractifyMap(cm[ck := cval], RefineKey, RefineValue, ReverseKey);
+            rm' == AbstractifyMap(cm, RefineKey, RefineValue, ReverseKey)[RefineKey(ck) := RefineValue(cval)];
+    ensures forall ck {:trigger RemoveElt(AbstractifyMap(cm, RefineKey, RefineValue, ReverseKey), RefineKey(ck)) } :: 
             (RefineKey.requires(ck) && ReverseKey.requires(RefineKey(ck)) && ReverseKey(RefineKey(ck)) == ck && ck in cm) ==>
-            var rm  := RefineToMap(cm, RefineKey, RefineValue, ReverseKey);
-            var rm' := RefineToMap(RemoveElt(cm, ck), RefineKey, RefineValue, ReverseKey);
+            var rm  := AbstractifyMap(cm, RefineKey, RefineValue, ReverseKey);
+            var rm' := AbstractifyMap(RemoveElt(cm, ck), RefineKey, RefineValue, ReverseKey);
             rm' == RemoveElt(rm, RefineKey(ck));
 {
-    lemma_RefineToMap_basic_properties(cm, RefineKey, RefineValue, ReverseKey);
-    lemma_RefineToMap_preimage(cm, RefineKey, RefineValue, ReverseKey);
+    Lemma_AbstractifyMap_basic_properties(cm, RefineKey, RefineValue, ReverseKey);
+    Lemma_AbstractifyMap_preimage(cm, RefineKey, RefineValue, ReverseKey);
 
     forall ck, cval | RefineKey.requires(ck) && RefineValue.requires(cval)
                    && ReverseKey.requires(RefineKey(ck)) && ReverseKey(RefineKey(ck)) == ck
-        ensures var rm  := RefineToMap(cm, RefineKey, RefineValue, ReverseKey);
-                var rm' := RefineToMap(cm[ck := cval], RefineKey, RefineValue, ReverseKey);
-                rm' == RefineToMap(cm, RefineKey, RefineValue, ReverseKey)[RefineKey(ck) := RefineValue(cval)];
+        ensures var rm  := AbstractifyMap(cm, RefineKey, RefineValue, ReverseKey);
+                var rm' := AbstractifyMap(cm[ck := cval], RefineKey, RefineValue, ReverseKey);
+                rm' == AbstractifyMap(cm, RefineKey, RefineValue, ReverseKey)[RefineKey(ck) := RefineValue(cval)];
     {
-        lemma_RefineToMap_append(cm, RefineKey, RefineValue, ReverseKey, ck, cval);
+        Lemma_AbstractifyMap_append(cm, RefineKey, RefineValue, ReverseKey, ck, cval);
     }
 
     forall ck | RefineKey.requires(ck) && ReverseKey.requires(RefineKey(ck)) && ReverseKey(RefineKey(ck)) == ck && ck in cm
-        ensures var rm  := RefineToMap(cm, RefineKey, RefineValue, ReverseKey);
-                var rm' := RefineToMap(RemoveElt(cm, ck), RefineKey, RefineValue, ReverseKey);
+        ensures var rm  := AbstractifyMap(cm, RefineKey, RefineValue, ReverseKey);
+                var rm' := AbstractifyMap(RemoveElt(cm, ck), RefineKey, RefineValue, ReverseKey);
                 rm' == RemoveElt(rm, RefineKey(ck));
     {
-        lemma_RefineToMap_remove(cm, RefineKey, RefineValue, ReverseKey, ck);
+        Lemma_AbstractifyMap_remove(cm, RefineKey, RefineValue, ReverseKey, ck);
     }
 
 }
