ironfleet/src/Dafny/Distributed/Impl/RSL/ReplicaModel-Part4.i.dfy
@@ -32,7 +32,7 @@ method Replica_Next_Process_AppStateRequest(
     var newExecutor, packets := ExecutorProcessAppStateRequest(replica.executor, inp, reply_cache_mutable);
     replica' := replica[executor := newExecutor];
     packets_sent := packets;
-    //lemma_RefineCPacketsToPacketsProperties(packets_sent);
+    //lemma_AbstractifySetOfCPacketsToSetOfRslPackets_properties(packets_sent);
     //lemma_AbstractifyCPacketToRslPacket_src(packets_sent, replica.constants.all.config.replica_ids[replica.constants.my_index]);
     var end_time := Time.GetDebugTimeTicks();
     RecordTimingSeq("Replica_Next_Process_AppStateRequest", start_time, end_time);
@@ -70,7 +70,7 @@ method Replica_Next_Process_Heartbeat(
     var newAcceptor := NextAcceptorState_ProcessHeartbeat(replica.acceptor, inp.msg, inp.src);
     replica' := replica[proposer := newProposer]
                        [acceptor := newAcceptor];
-    //lemma_RefineCPacketsToPacketsProperties(packets_sent);
+    //lemma_AbstractifySetOfCPacketsToSetOfRslPackets_properties(packets_sent);
     var end_time := Time.GetDebugTimeTicks();
     RecordTimingSeq("Replica_Next_Process_Heartbeat", start_time, end_time);
 
@@ -105,7 +105,7 @@ method {:timeLimitMultiplier 2} Replica_Next_ReadClock_CheckForViewTimeout(
     packets_sent := Broadcast(CBroadcastNop);
     assert OutboundPacketsIsValid(packets_sent);
     assert OutboundPacketsHasCorrectSrc(packets_sent, replica.constants.all.config.replica_ids[replica.constants.my_index]);
-    //lemma_RefineCPacketsToPacketsProperties(packets_sent);
+    //lemma_AbstractifySetOfCPacketsToSetOfRslPackets_properties(packets_sent);
     var end_time := Time.GetDebugTimeTicks();
     RecordTimingSeq("Replica_Next_ReadClock_CheckForViewTimeout", start_time, end_time);
 
@@ -139,7 +139,7 @@ method {:timeLimitMultiplier 2} Replica_Next_ReadClock_CheckForQuorumOfViewSuspi
     packets_sent := Broadcast(CBroadcastNop);
     assert OutboundPacketsIsValid(packets_sent);
     assert OutboundPacketsHasCorrectSrc(packets_sent, replica.constants.all.config.replica_ids[replica.constants.my_index]);
-    //lemma_RefineCPacketsToPacketsProperties(packets_sent);
+    //lemma_AbstractifySetOfCPacketsToSetOfRslPackets_properties(packets_sent);
     var end_time := Time.GetDebugTimeTicks();
     RecordTimingSeq("Replica_Next_ReadClock_CheckForQuorumOfViewSuspicions", start_time, end_time);
 
